

* AP & GP fundamental *

Page: WABER

Date: 10/11/2024

* Sequence *

→ collection of elements is ordered in such a way that it has to an identified 1st member, 2nd member

→ if sequence follows a specific pattern then it is known as progression

ex.

1, 2, 3, 4, 5, ...	$2-1=3-2=4-3$	} A.P.
2, 4, 6, 8, 10, ...	$4-2=6-4=8-6$	
3, 6, 9, 12, 15, ...	$6-3=9-6=12-9$	
2, 4, 8, 16, 32, ...	$4/2=8/4=16/8$	} G.P.
3, 9, 27, 81, ...	$9/3=27/9=81/27$	

(1) A.P. (Arithmetic Progression)

~~a~~

$$a, a+d, a+2d, a+3d, a+4d, \dots, a+(n-1)d$$

↓	↓	↓	↓	↓	↓
1 st	2 nd	3 rd	4 th	5 th	n th term

→ nth term of AP = $a + (n-1)d$

d → common difference

* Series *

→ if $a_1, a_2, a_3, a_4, \dots, a_n$ be the sequence then the expression $a_1 + a_2 + a_3 + a_4 + \dots + a_n$ is called series associated with sequence

$1, 2, 3, 4, 5 \rightarrow$ sequence

$1 + 2 + 3 + 4 + 5 \rightarrow$ series

$15 \rightarrow$ sum of series

* sum of n terms of A.P. series *

$$S_n = a + a+d + a+2d + a+3d + \dots + a+(n-1)d$$

$$\text{last term} = a+(n-1)d = L$$

$$2^{\text{nd}} \text{ last term} = a+(n-2)d = L-d$$

$$3^{\text{rd}} \text{ last term} = a+(n-3)d = L-2d$$

$$S_n = a + a+d + a+2d + \dots + L-2d + L-d + L \quad \text{--- (1)}$$

$$S_n = L + L-d + L-2d + \dots + a+2d + a+d + a \quad \text{--- (2)}$$

\rightarrow add both equation

$$2S_n = (a+L) + (a+L) + (a+L) + \dots + (a+L)$$

$$2S_n = n \cdot (a+L)$$

$$S_n = \frac{n}{2} (a+L)$$

$$S_n = \frac{n}{2} (a + [a+(n-1)d])$$

(2) G.P. (Geometric Progression)

$$a, ar, ar^2, ar^3, ar^4, \dots, ar^{n-1}$$

$$\downarrow \quad \downarrow \quad \downarrow \quad \downarrow \quad \downarrow \quad \downarrow$$

$$1^{st} \quad 2^{nd} \quad 3^{rd} \quad 4^{th} \quad 5^{th} \quad n^{th}$$

→ n^{th} term of GP = ar^{n-1}

* Sum of n term of G.P. series *

$$S_n = a + ar + ar^2 + ar^3 + ar^4 + \dots + ar^{n-1} \quad \text{--- (1)}$$

$$r * S_n = ar + ar^2 + ar^3 + ar^4 + ar^5 + \dots + ar^{n-1} + ar^n \quad \text{--- (2)}$$

→ now subtract both equation.

$$S_n(1-r) = a - ar^n$$

$$S_n = \frac{a - ar^n}{1-r}$$

$$S_n = \frac{a(1-r^n)}{1-r} = - \frac{a(r^n-1)}{-(r-1)} = \frac{a(r^n-1)}{r-1}$$

$$r < 1$$

$$S_\infty = \frac{a[1-0]}{1-r} = \frac{a}{1-r}$$

Q. $1 + 2 + 3 + 4 + \dots + n$ [sum of 1st n natural no.]

→ This is A.P. series so,

$$\begin{aligned} S_n &= \frac{n}{2} [2a + (n-1)d] \\ &= \frac{n}{2} [2 + (n-1)1] \\ &= \frac{n}{2} (n+1) \\ &= \frac{n(n+1)}{2} \end{aligned}$$

Q. $1 + 3 + 5 + 7 + \dots$ [sum of odd natural numbers]

→

$$\begin{aligned} S_n &= \frac{n}{2} [2a + (n-1)d] \\ &= \frac{n}{2} [2 + (n-1)2] \\ &= \frac{n}{2} [2 + 2n - 2] \\ &= \frac{n}{2} \times 2n \\ &= n^2 \end{aligned}$$

Q. $2 + 4 + 6 + 8 + 10 + \dots$ [sum of even natural no.]

→

$$\begin{aligned} S_n &= \frac{n}{2} [2a + (n-1)d] \\ &= \frac{n}{2} [2 \times 2 + (n-1)2] \\ &= \frac{n}{2} [4 + 2n - 2] \\ &= \frac{n}{2} [2 + 2n] \Rightarrow \frac{n}{2} \times 2(n+1) \Rightarrow n(n+1) \end{aligned}$$

Q. $1^2 + 2^2 + 3^2 + 4^2 + 5^2 + \dots$ [sum of square of natural number]

→

$$S_n = \frac{n}{2} [2a + (n-1)d]$$

$$= \frac{n}{2} [2a + (n-1)d]$$

$$(x+1)^3 - x^3 = x^3 + 3x^2 + 3x + 1 - x^3$$

$$= 1 + 3x + 3x^2$$

$$x = 1$$

$$2^3 - 1^3 = 1 + 3 \times 1 + 3 \times 1^2 \quad \text{--- (1)}$$

$$x = 2$$

$$3^3 - 2^3 = 1 + 3 \times 2 + 3 \times 2^2 \quad \text{--- (2)}$$

$$x = n$$

$$(n+1)^3 - n^3 = 1 + 3n + 3n^2 \quad \text{--- (3)}$$

→ now sum all these equation.

$$(n+1)^3 - 1^3 = 3 [1^2 + 2^2 + 3^2 + \dots + n^2] + 3 [1 + 2 + 3 + \dots + n]$$

$$= 3 \sum n^2 + \frac{3n(n+1)}{2} + n$$

$$3 \sum n^2 = (n+1)^3 - 1 - \frac{3n(n+1)}{2} - n$$

$$= (n+1) \left[(n+1)^2 - \frac{3n}{2} \right] - [n+1]$$

$$= (n+1) \left[(n+1)^2 - \frac{3n}{2} - 1 \right]$$

$$= (n+1) \left(n^2 + 2n + 1 - \frac{3n}{2} - 1 \right)$$

$$= (n+1) \left(n^2 + \frac{n}{2} \right)$$

$$\Rightarrow 3 \sum n^2 = (n+1)(n) \frac{(2n+1)}{2}$$

$$= \sum n^2 = \frac{n(n+1)(2n+1)}{6}$$

Q. $1^3 + 2^3 + 3^3 + \dots$ [sum of squares of natural number]

→

$$(x+1)^4 - x^4$$

$$(a+b)^n = \sum_{r=0}^n {}^nC_r a^r b^{n-r} = {}^nC_0 a^0 b^n + {}^nC_1 a^1 b^{n-1} + {}^nC_2 a^2 b^{n-2} + \dots + {}^nC_n a^n b^0$$

$$(x+1)^n = \sum_{r=0}^n {}^nC_r x^r = {}^nC_0 x^0 + {}^nC_1 x^1 + {}^nC_2 x^2 + \dots + {}^nC_n x^n$$

$$(x+1)^4 - x^4 = {}^4C_0 x^0 + {}^4C_1 x^1 + {}^4C_2 x^2 + {}^4C_3 x^3 + {}^4C_4 x^4 - x^4$$

$$= 1 + 4x + 6x^2 + 4x^3 + x^4 - x^4$$

$$= 4x^3 + 6x^2 + 4x + 1$$

$$x = 1$$

$$2^4 - 1^4 = 4 \times 1^3 + 6 \times 1^2 + 4 \times 1 + 1$$

$$x = 2$$

$$3^4 - 2^4 = 4 \times 2^3 + 6 \times 2^2 + 4 \times 2 + 1$$

$$x = n$$

$$4n^3 + 6n^2 + 4n + 1$$

$$(n+1)^4 - n^4 = 4[1^3 + 2^3 + 3^3 + \dots + n^3] + 6[1^2 + 2^2 + 3^2 + \dots + n^2] + 4[1 + 2 + 3 + \dots + n] + 1 + 1 + 1$$

$$(n+1)^4 - n^4 = 4 \sum n^3 + 6 \sum n^2 + 4 \sum n + 1$$

$$4 \sum n^3 = (n+1)^4 - n^4 - 6 \sum n^2 - 4 \sum n - 1$$

$$= (n+1)^4 - 1 - 6n(n+1)(2n+1) - \frac{4 \times n(n+1)(n+2)}{2}$$

$$= (n+1)^4 - 1 - n(n+1)(2n+1) - 2n(n+1) - n$$

$$= n+1 [(n+1)^3 - n(2n+1) - 2n] - (n+1)$$

$$= n+1 [(n+1)^3 - n(2n+1) - 2n - 1]$$

$$\begin{aligned}
 &= (n+1) [n^3 + 1 + 3n(n+1) - 2n^2 - n - 2n - 1] \\
 &= (n+1) [n^3 + 3n^2 + 3n - 2n^2 - 3n] \\
 &= (n+1) [n^3 + n^2] \\
 &= (n+1) (n^2) (n+1)
 \end{aligned}$$

$$\sum n^3 = \frac{(n+1)^2 (n^2)}{4}$$

$$= \left(\frac{(n+1)(n)}{2} \right)^2$$

Q. In an AP 7th term is 40 & 24th term is 124 find 31th term

→

$$n^{\text{th}} \text{ term} = a + (n-1)d$$

$$7^{\text{th}} = a + 6d = 40 \quad \text{--- (1)}$$

$$24^{\text{th}} = a + 23d = 124 \quad \text{--- (2)}$$

$$a + 6d = 40$$

$$a + 23d = 124$$

$$- 17d = -84$$

$$d = 6$$

→ Put value of d is (1)

$$a + 36 = 40$$

$$a = 4$$

for 31th term $a = 4$, $d = 6$, $n = 31$

$$= 4 + 30 \times 6$$

$$= 4 + 180$$

$$= 184$$

Q. Sum of series $10 + 84 + 734 + \dots =$

$$\rightarrow (a^1 + 1) + (a^2 + 3) + (a^3 + 5) + \dots$$

$$\underbrace{(a^1 + a^2 + a^3 + \dots)}_{\text{G.P.}} + (1 + 3 + 5 + \dots)$$

$$= \frac{a(a^n - 1)}{a - 1} + n^2$$

$$= \frac{a^{n+1} - a}{8} + n^2$$

$$= \frac{a^{n+1} + 8n^2 - a}{8}$$

Q. $11 + 111 + 1111 + \dots + n$

\rightarrow

$$11 [1 + 11 + 111 + \dots + n]$$

$$\frac{11}{11} [a + aa + aaa + \dots + n]$$

$$\frac{11}{11} [(10^1 - 1) + (10^2 - 1) + (10^3 - 1) + \dots + n]$$

$$\frac{11}{11} [(10^1 + 10^2 + 10^3 + \dots + 10^n) - n]$$

$$\frac{11}{11} \left[10 \frac{(10^n - 1)}{10 - 1} - n \right]$$

$$= \frac{4}{4} \left[\frac{10^{n+1} - 10 - 4n}{4} \right]$$

$$= \frac{4}{4} \left[10^{n+1} - 4n - 10 \right]$$

Q. A ball is dropped from 400m & every time it becomes to $\frac{2}{3}$ rd of its height. find total distance covered by ball before comming to rest

→

$$= 400 + 2 \times \frac{2}{3} \times 400 + 2 \times \left(\frac{2}{3}\right)^2 \times 400$$

$$= 400 \left[1 + 2 \times \frac{2}{3} + 2 \times \left(\frac{2}{3}\right)^2 + \dots \right]$$

$$= 400 \left[1 + 2 \left[\frac{2}{3} + \left(\frac{2}{3}\right)^2 + \dots \right] \right]$$

→ here $r < 1$

$$S_{\infty} = \frac{a}{1-r}$$

$$= 400 \left[1 + 2 \left[\frac{2/3}{1/3} \right] \right]$$

$$= 400 [5]$$

$$= 4500 \text{ m}$$